# implication $(E+F)*\Rightarrow(E*F*)*$
Soit $(E+F)*=(E*\times F*)*$
- Soit $w =w_{1}w_{2},w_{3},\dots w_{n}\in(E+F)*$, alors pour tout $i$ on a $w_{i}=E$ ou $w_{i}=F$
- Dans tous les cas on a $w_{i}\in(E*F*)$, alors $w \in (E*F*)*$
# Implication $(E+F)*\Leftarrow(E*F*)*$
- Soit $w=w_{1},w_{2},w_{3},\dots,w_{n}\in(E*F*)*$, alors pour tout $i$ on a $w_{i}=E_{j}F_{k}=xy$ tel que $x \in (E+F)*$ et $y=(E+F)*$
- Ainsi, $x,y \in (E+F)*(E+F)=(E+F)*$
- Ainsi, $w=w_{1},w_{2}\dots w_{n} \in ((E+F)*)*=(E+F)*$
